\documentclass[12pt]{article}
\usepackage{cmap}
\usepackage[utf8]{inputenc}
\usepackage[russian]{babel}
\begin{document}

\section*{Вычисление производных.}

Заметим, что
\\
$ d y_1 y_2 = \frac{ (c_{22}c_{13} - c_{12}c_{23}) (c_{11}c_{23} - c_{21}c_{13}) }{d} = \frac{ c_{22}c_{13}c_{11}c_{23} + c_{12}c_{23}c_{21}c_{13} }{d} = c_{13}c_{23}, $
\\
$ d c_{31} y_1 c_{32} y_2 = - c_{31}c_{32} d y_1 y_2 = - c_{31}c_{32}c_{13}c_{23} = c_{31}c_{13}c_{32}c_{23}, $
\\
$ c_{13} (c_{31} y_1 + c_{32} y_2) = \frac{c_{13}c_{31} (c_{22}c_{13} - c_{12}c_{23}) + c_{13}c_{32} (c_{11}c_{23} - c_{21}c_{13}) }{d} = \frac{-c_{13}c_{23} (c_{32}c_{11} - c_{31}c_{12})}{d} = c_{11} c_{32} y_2 y_1 + c_{12}c_{31} y_1 y_2, $
\\
$ c_{11} y_1 + c_{12} y_2 = \frac{c_{11} (c_{22}c_{13} - c_{12}c_{23}) + c_{12} (c_{11}c_{23} - c_{21}c_{13}) }{d} = 
\frac{ c_{11}c_{22}c_{13} - c_{12}c_{21}c_{13} }{d} = c_{13}. $
\\

\input{derivatives_full/d_dy}

Запишем базисные векторы в виде
\\
$ v_i = d^{\lambda_2 - 1} c_{11}^{\lambda_1 - \lambda_2 - i} c_{12}^i (c_{33}^{\lambda_3} d - \lambda_3 c_{33}^{\lambda_3 - 1} (c_{31} d y_1 + c_{32} d y_2) + \lambda_3 (\lambda_3 - 1) c_{33}^{\lambda_3 - 2} c_{31}c_{13}c_{32}c_{23}), $
\\
$ w_i = d^{\lambda_2 - 1} c_{11}^{\lambda_1 - \lambda_2 - i} c_{12}^i (c_{33}^{\lambda_3} d y_1 - \lambda_3 c_{33}^{\lambda_3 - 1} c_{32}c_{23}c_{13}), $
\\
$ u_i = d^{\lambda_2 - 1} c_{11}^{\lambda_1 - \lambda_2 - i} c_{12}^i (c_{33}^{\lambda_3} d y_2 - \lambda_3 c_{33}^{\lambda_3 - 1} c_{31}c_{13}c_{23}), $
\\
$ r_i = d^{\lambda_2 - 1} c_{11}^{\lambda_1 - \lambda_2 - i} c_{12}^i c_{33}^{\lambda_3} c_{13}c_{23}. $
\newline

\input{derivatives_full/vi}
\newline

\input{derivatives_full/wi}
\newline

\input{derivatives_full/ui}
\newline

\input{derivatives_full/ri}

\end{document}
